Delimited release example.

theories/examples/calendar.v
@@ -1,3 +1,7 @@
+(** This example demonstrates and approach to handling delimited information release in SeLoC.
+
+It is based on the example from  "A Separation Logic for Enforcing DeclarativeInformation Flow Control Policies" by David Costanzo and Zhong Shao.
+*)
 From iris.base_logic Require Import invariants.
 From iris_ni.logrel Require Import types.
 From iris_ni.program_logic Require Import dwp heap_lang_lifting.
@@ -7,9 +11,56 @@ From iris_ni.proofmode Require Import dwp_tactics.
 From iris_ni.logrel Require Import interp.
 From iris_ni.examples Require Import lock.
 
+(** The idea behind this example, is that a person A. has a calendar,
+(which we model as a linked list), and each day is marked eiter with 0
+(meaining that the day is free, and there are no meetings) or with a
+positive integer t (meatning that there is a meeting at time t).
+
+If someone wants to set up their appointment with A., they have to see
+which days are they available. In order to do so, A. must be able to
+disclose the days on which they are free, without disclosing any other
+information (e.g. times of other meetings).
+
+The program that discloses the avilablility of A. is the
+`available_dates` below.
+
+We show non-interference with a form of delimited control.
+Specifically, we show that if an attacker already knows the days on
+which A. is available, then the attacker cannot learn any further
+information.
+ *)
+
+(* Iterate a function `f` over the linked list `hd`
+   `f` is called with `f i x` where `x` is `i`-th element in the list.
+ *)
+Definition iter_loop : val :=
+  rec: "loop" "i" "hd" "f" :=
+    match: "hd" with
+      NONE => #()
+    | SOME "l" =>
+      let: "tmp1" := Fst !"l" in
+      let: "tmp2" := Snd !"l" in
+      "f" "i" "tmp1";;
+      "loop" ("i"+#1) "tmp2" "f"
+    end.
+Definition iter : val := λ: "hd" "f", iter_loop #0 "hd" "f".
+
+
+Definition available_dates (out : loc) : val := λ: "cal",
+  iter "cal" (λ: "i" "x", if: "x" = #0 then #out <- "i" else Skip).
+
+(* Meta-function (macro) : create a HeapLang linked list out of a Coq list *)
+Fixpoint make_llist (xs : list val) : expr :=
+  match xs with
+  | [] => NONE
+  | (x::xs) =>
+    SOME (ref (x, make_llist xs))
+  end.
+
 Section calendar.
   Context `{!heapDG Σ}.
 
+  (* Predicate describing that `hd1` and `hd2` point to lists `xs1` and `xs2`, respectively *)
   Fixpoint is_list (hd1 : val) (hd2 : val) (xs1 xs2 : list val) : iProp Σ :=
     match xs1,xs2 with
     | [],[] => ⌜hd1 = NONEV⌝ ∗ ⌜hd2 = NONEV⌝
@@ -19,33 +70,101 @@ Section calendar.
     | _, _ => False
     end%I.
 
-  Definition iter : val := rec: "loop" "hd" "f" :=
-      match: "hd" with
-        NONE => #()
-      | SOME "l" =>
-         let: "tmp1" := Fst !"l" in
-         let: "tmp2" := Snd !"l" in
-         "f" "tmp1";;
-         "loop" "tmp2" "f"
-      end.
+  Lemma make_llist_spec (xs1 xs2 : list val) :
+    length xs1 = length xs2 →
+    ⊢ DWP make_llist xs1 & make_llist xs2 : λ hd1 hd2, is_list hd1 hd2 xs1 xs2.
+  Proof using Type.
+    revert xs2. induction xs1 as [|x1 xs1]=>xs2; simpl.
+    - intros Hxs2. symmetry in Hxs2. eapply nil_length_inv in Hxs2.
+      simplify_eq/=. dwp_pures.
+      iApply dwp_value. eauto.
+    - destruct xs2 as [|x2 xs2]; simpl.
+      { inversion 1. }
+      intros Hlen. simplify_eq/=.
+      dwp_bind (make_llist xs1) (make_llist xs2).
+      iApply (dwp_wand with "[]").
+      { by iApply IHxs1. }
+      iIntros (t1 t2) "Ht". dwp_pures.
+      dwp_bind (ref _)%E (ref _)%E.
+      iApply dwp_alloc. iIntros (hd1 hd2) "Hhd1 Hhd2". iNext.
+      dwp_pures. iApply dwp_value. iModIntro.
+      iExists _,_,_,_. eauto with iFrame.
+  Qed.
 
-  Lemma iter_spec P (f1 f2 :val) hd1 hd2 xs1 xs2 ξ :
+  (* Specifications for the iter function *)
+  Lemma iter_loop_spec P (i : Z) (f1 f2 :val) hd1 hd2 xs1 xs2 ξ :
     Forall2 P xs1 xs2 →
     is_list hd1 hd2 xs1 xs2 -∗
-    □(∀ x1 x2, ⌜P x1 x2⌝ → DWP (App f1 x1) & (App f2 x2) : ⟦ tunit ⟧ ξ) -∗
-    DWP iter hd1 f1 & iter hd2 f2 : ⟦ tunit ⟧ ξ.  (* TODO: return is_list *)
-  Proof.
+    □(∀ x1 x2 (i : Z), ⌜P x1 x2⌝ → DWP (App f1 #i x1) & (App f2 #i x2) : ⟦ tunit ⟧ ξ) -∗
+    DWP iter_loop #i hd1 f1
+      & iter_loop #i hd2 f2 : ⟦ tunit ⟧ ξ.
+  Proof using Type.
     iIntros (Hxs) "Hlst #Hf". iRevert (Hxs).
-    iLöb as "IH" forall (hd1 hd2 xs1 xs2). iIntros (Hxs).
+    iLöb as "IH" forall (i hd1 hd2 xs1 xs2). iIntros (Hxs).
     dwp_rec. dwp_pures.
     destruct xs1 as [|x1 xs1], xs2 as [|x2 xs2]; iSimpl in "Hlst"; try by iExFalso.
     - iDestruct "Hlst" as "[-> ->]". dwp_pures. iApply logrel_unit.
     - iDestruct "Hlst" as (l1 l2 hd1' hd2' -> ->) "(Hl1 & Hl2 & Hlst)".
-      apply Forall2_cons_inv in Hxs.
+      apply Forall2_cons_inv in Hxs. destruct Hxs.
       dwp_pures. dwp_bind (! _)%E (! _)%E. iApply (dwp_load with "Hl1 Hl2"). iIntros "Hl1 Hl2". iNext.
       dwp_pures. dwp_bind (! _)%E (! _)%E. iApply (dwp_load with "Hl1 Hl2"). iIntros "Hl1 Hl2". iNext.
-      dwp_pures. dwp_bind (f1 x1) (f2 x2). iApply (dwp_wand with "[Hf]").
+      dwp_pures. dwp_bind (f1 #i x1) (f2 #i x2). iApply (dwp_wand with "[Hf]").
       { iApply "Hf". iPureIntro. naive_solver. }
-      iIntros (??) "_". dwp_pures. iApply ("IH" with "Hlst"). naive_solver.
+      iIntros (??) "_". dwp_pures.
+      iApply ("IH" $! (i+1)%Z with "Hlst [%//]").
   Qed.
+
+  Lemma iter_spec P (f1 f2 :val) hd1 hd2 xs1 xs2 ξ :
+    Forall2 P xs1 xs2 →
+    is_list hd1 hd2 xs1 xs2 -∗
+    □(∀ x1 x2 (i : Z), ⌜P x1 x2⌝ → DWP (App f1 #i x1) & (App f2 #i x2) : ⟦ tunit ⟧ ξ) -∗
+    DWP iter hd1 f1 & iter hd2 f2 : ⟦ tunit ⟧ ξ.  (* TODO: return is_list *)
+  Proof using Type.
+    iIntros (Hxs) "Hlst #Hf". dwp_rec. dwp_pures.
+    iApply (iter_loop_spec with "Hlst Hf"); eauto.
+  Qed.
+
+  Lemma available_dates_spec (out : loc) hd1 hd2 xs1 xs2 :
+    Forall2 (λ x1 x2, x1 = #0 ↔ x2 = #0) xs1 xs2 →
+    ⟦ tref (tint Low) ⟧ Low #out #out -∗
+    is_list hd1 hd2 xs1 xs2 -∗
+    DWP available_dates out hd1 & available_dates out hd2 : ⟦ tunit ⟧ Low.
+  Proof using Type.
+    iIntros (HP) "#Hout Hlst". dwp_rec. dwp_pures.
+    iApply (iter_spec with "Hlst [-]"); eauto.
+    iModIntro. iIntros (x1 x2 i Hxs).
+    dwp_pures.
+    case_bool_decide; case_bool_decide; try by (exfalso; naive_solver).
+    - dwp_pures.
+      iApply logrel_store ; eauto; iApply dwp_value; eauto.
+      iModIntro. iExists _,_. eauto.
+    - dwp_pures. iApply logrel_unit.
+  Qed.
+
 End calendar.
+
+From iris_ni Require Import program_logic.dwp_adequacy.
+
+(* Adequacy statement *)
+(* xs1 xs2 are calendars *)
+Lemma available_dates_secure (out : loc) (xs1 xs2 : list val) σ1 σ2 (n : Z):
+    Forall2 (λ x1 x2, x1 = #0 ↔ x2 = #0) xs1 xs2 →
+    σ1.(heap) !! out = Some (Some #n) →
+    σ2.(heap) !! out = Some (Some #n) →
+    dwp_adequacy.R heapDΣ {[out]}
+                   ([let: "hd1" := make_llist xs1 in available_dates out "hd1"]%E,σ1)
+                   ([let: "hd2" := make_llist xs2 in available_dates out "hd2"]%E,σ2).
+Proof using Type.
+  intros Hxs Hσ1 Hσ2.
+  apply tc_once. simpl.
+  eapply dwp_lift_bisim_singleton; eauto.
+  iIntros (HG) "Ho".
+  dwp_bind (make_llist xs1) (make_llist xs2).
+  iApply (dwp_wand with "[]").
+  { iApply make_llist_spec. by eapply Forall2_length. }
+  iIntros (hd1 hd2) "Hhd". dwp_pures.
+  iApply (dwp_wand with "[-]").
+  { by iApply (available_dates_spec with "Ho Hhd"). }
+  iIntros (v1 v2). iDestruct 1 as "[-> ->]".
+  eauto.
+Qed.
